Prove typed wp_load

src/new_goose_lang/lib/typed_mem/impl.v
@@ -6,40 +6,46 @@ Reserved Notation "![ t ] e"
 Reserved Notation "e1 <-[ t ] e2"
          (at level 80, format "e1  <-[ t ]  e2").
 
+Inductive go_abstract_type :=
+| cellT
+| unitT
+| prodT (t1 t2 : go_abstract_type)
+.
+Fixpoint go_abstract_type_size (t : go_abstract_type) : nat :=
+  match t with
+  | prodT t1 t2 => go_abstract_type_size t1 + go_abstract_type_size t2
+  | cellT => 1
+  | unitT => 0
+  end.
+
+Fixpoint go_type_interp (t : go_type) : go_abstract_type :=
+  match t with
+  | sliceT _ => prodT (prodT (prodT cellT cellT) cellT) unitT
+  | structT decls => fold_right prodT unitT (fmap (go_type_interp ∘ snd) decls)
+  | interfaceT => prodT (prodT (prodT cellT cellT) cellT) unitT (* type id, val, methods *)
+  | _ => cellT
+  end.
+
+Definition go_type_size (t : go_type) : nat := go_abstract_type_size $ go_type_interp t.
+
+
+Reserved Notation "l +ₗ[ t ] z" (at level 50, left associativity, format "l  +ₗ[ t ]  z").
+Notation "l +ₗ[ t ] z" := (l +ₗ go_abstract_type_size (go_type_interp t) * z) : stdpp_scope .
+Notation "e1 +ₗ[ t ] e2" := (BinOp (OffsetOp (go_abstract_type_size $ go_type_interp t)) e1%E e2%E) : expr_scope .
+
 Section go_lang.
   Context `{ffi_syntax}.
 
   (** allocation with a type annotation *)
   Definition ref_to (t:go_type): val := λ: "v", ref (Var "v").
 
-  Inductive go_abstract_type :=
-  | cellT
-  | unitT
-  | prodT (t1 t2 : go_abstract_type)
-  .
-  Fixpoint go_abstract_type_size (t : go_abstract_type) : nat :=
-    match t with
-    | prodT t1 t2 => go_abstract_type_size t1 + go_abstract_type_size t2
-    | cellT => 1
-    | unitT => 0
-    end.
-
-  Fixpoint go_type_interp (t : go_type) : go_abstract_type :=
-    match t with
-    | sliceT _ => prodT (prodT (prodT cellT cellT) cellT) unitT
-    | structT decls => fold_right prodT unitT (fmap (go_type_interp ∘ snd) decls)
-    | interfaceT => prodT (prodT (prodT cellT cellT) cellT) unitT (* type id, val, methods *)
-    | _ => cellT
-    end.
-
-  Definition go_type_size (t : go_type) : nat := go_abstract_type_size $ go_type_interp t.
-
   (* TODO: seal *)
   Definition load_ty (t : go_type) : val :=
     (fix load_ty_aux t : val :=
       match t with
       | prodT t1 t2 => (λ: "l", (load_ty_aux t1 (Var "l"),
-                                  load_ty_aux t2 (Var "l" +ₗ #(go_abstract_type_size t1))))%V
+                                  load_ty_aux t2 (BinOp (OffsetOp (go_abstract_type_size t1))
+                                                                  (Var "l") #1)))%V
       | cellT => (λ: "l", !(Var "l"))%V
       | unitT => (λ: <>, #())%V
       end) (go_type_interp t).
@@ -69,7 +75,3 @@ Notation "![ t ] e" := (load_ty t e%E) : expr_scope.
    trick. *)
 Notation "e1 <-[ t ] e2" := (store_ty t (Pair e1%E e2%E)) : expr_scope.
 Notation "v1 <-[ t ] v2" := (store_ty t (PairV v1%V v2%V)) : val_scope.
-
-Reserved Notation "l +ₗ[ t ] z" (at level 50, left associativity, format "l  +ₗ[ t ]  z").
-Notation "l +ₗ[ t ] z" := (l +ₗ go_abstract_type_size (go_type_interp t) * z) : stdpp_scope .
-Notation "e1 +ₗ[ t ] e2" := (BinOp (OffsetOp (go_abstract_type_size $ go_type_interp t)) e1%E e2%E) : expr_scope .
